proof/gate.ec
@@ -2,20 +2,12 @@ require import Bitstring.
 require import Int.
 require import Map.
 require import Pair.
-require import Scheme.
 require import Dkc.
+require import GarbleTools.
+require import Bool.
 
-op lsb(b:bitstring) : bool = b.[0].
-
-op fst(x:'a*'b*'c) : 'a = let (a, b, c) = x in a.
-op snd(x:'a*'b*'c) : 'b = let (a, b, c) = x in b.
-op thi(x:'a*'b*'c) : 'c = let (a, b, c) = x in c.
-
-type token = Dkc.number.
-type tokens = (int*bool, token) map.
-
-op tweak(a:bool, b:bool) : bitstring = a::(b::(zeros (Scheme.k-2))).
-
+(*
+require import Scheme.
 clone Scheme as Gate with
   type funct = bool*bool*bool*bool,
   type functG = token*token*token*token,
@@ -26,123 +18,68 @@ clone Scheme as Gate with
   type inputG = token*token,
   type outputG = bool,
   type random = tokens.
+*)
 
-(*
 theory Gate.
-  type token = Dkc.number.
-  type tokens = (int*bool, Gate.token) map.
 
   type funct = bool*bool*bool*bool.
   type functG = token*token*token*token.
   type input = bool*bool.
   type output = bool.
-  type keyInput = token*token*token*token.
+  type keyInput = tokens.
   type keyOutput = unit.
   type inputG = token*token.
-  type outputG = bool.
-  
-  op eval(f:funct, i:input) : output =
-    let (ff, ft, tf, tt) = f in
-    let (i1, i2) = i in
-    if !i1 && !i2 then ff else
-    if !i1 && i2 then ft else
-    if  i1 && !i2 then tf else
-    tt.
+  type outputG = token.
+  type phiT = unit.
 
-  op enc(x:tokens, f:funct, x1:bool, x2:bool) : token =
-    let xx1 = (lsb (proj x.[(1, true)]) = x1) in
-    let xx2 = (lsb (proj x.[(2, true)]) = x2) in
-    Dkc.encode
-      (tweak x1 x2)
-      (proj x.[(1, xx1)])
-      (proj x.[(2, xx2)])
-      (proj x.[(3, eval f (xx1,xx2))]).
+  op phi : phiT = tt.
+
+  op eval(f:funct, i:input) : output = evalGate f i.
+
   op _garble(x:tokens, f:funct) : functG*keyInput*keyOutput =
-    (
-      (enc x f false false, enc x f false true, enc x f true false, enc x f true true),
-      (proj x.[(1, false)], proj x.[(1, true)], proj x.[(2, false)], proj x.[(2, true)]),
-      tt
-    ).
-  pred tokenCorrect(x:tokens) =
-    (lsb (proj x.[(1, false)]) <> lsb (proj x.[(1, true)])) /\
-    (lsb (proj x.[(2, false)]) <> lsb (proj x.[(2, true)])) /\
-    (lsb (proj x.[(3, false)]) = false) /\
-    (lsb (proj x.[(3, true )]) = true).
+    (garbleGate x f 0 1 2, x, tt).
+  
+  pred tokenCorrect(x:tokens) = tokenCorrect 2 1 1 x.
 
   op encrypt(k:keyInput, i:input) : inputG =
-    let (f1, t1, f2, t2) = k in
-    let x1 = if fst i then t1 else f1 in
-    let x2 = if snd i then t2 else f2 in
-    (x1, x2).
+    (getTok k 0 (fst i), getTok k 1 (snd i)).
 
-  op decrypt(k:keyOutput, o:outputG) : output = o.
+  op decrypt(k:keyOutput, o:outputG) : output = lsb o.
 
   op evalG(g:functG, i:inputG) : outputG =
-    let (ff, ft, tf, tt) = g in
     let a = lsb (fst i) in
     let b = lsb (snd i) in
-    let t =
-      if !a && !b then ff else
-      if !a &&  b then ft else
-      if  a && !b then tf else
-      tt in
-    lsb (Dkc.decode (tweak a b) (fst i) (snd i) t).
-
-  lemma oparg :
-    forall (f : 'a -> 'b),
-    forall (x : 'a),
-    forall (y : 'a),
-      (x = y) => (f x = f y).
+    let t = evalGate g (a, b) in
+    Dkc.decode (tweak 2 a b) (fst i) (snd i) t.
 
   lemma inverse :
     forall (i : input) ,
     forall (f : funct) ,
     forall (x : tokens) ,
-     let i1 = fst i in
-     let i2 = snd i in
       tokenCorrect x =>
-      let temp = _garble x f in
-      let g = fst temp in
-      let ki = snd temp in
-      let ko = thi temp in
-      eval f (i1, i2) = decrypt ko (evalG g (encrypt ki (i1, i2)))
+      let (g, ki, ko) = _garble x f in
+      eval f i = decrypt ko (evalG g (encrypt ki i))
   proof.
-
-  intros i f x i1 i2 tC g ki ko;
-  delta decrypt evalG encrypt g ki ko tC _garble Pair.fst Pair.snd fst snd.
-
-  case (i1).
-  case (i2).
-
+  intros i f x.
+  intros tokCor.
+  cut main : (
+    let (g, ki, ko) = _garble x f in
+    evalG g (encrypt ki i) = getTok x 2 (eval f i)
+  ).
+  delta _garble decrypt eval evalG encrypt.
   simplify.
-  case (lsb (proj x.[(1, true)])).
-  simplify.
+  apply (inverse_base i 2 1 1 0 1 2 f x _ _ _ _ _ _ _).
   trivial.
-  simplify.
   trivial.
-
-  simplify.
-  case (lsb (proj x.[(1, true)])).
-  simplify.
   trivial.
-  simplify.
   trivial.
-
-  case (i2).
-
-  simplify.
-  case (lsb (proj x.[(1, false)])).
-  simplify.
   trivial.
-  simplify.
   trivial.
-
-  simplify.
-  case (lsb (proj x.[(1, false)])).
-  simplify.
   trivial.
-  simplify.
+  cut main2 : (let (g, ki, ko) = _garble x f in
+    eval f i = decrypt ko (getTok x 2 (eval f i))).
+  trivial.
   trivial.
   save.
 
-end Gate.*)
+end Gate.
