proof/myTools.ec
@@ -1,0 +1,177 @@
+require import Int.
+require import Array.
+
+lemma strongInduction:
+  forall (p:int -> bool),
+    (forall j, 0 <= j => (forall k, k >= 0 => k < j => p k) => p j) =>
+      (forall i, 0 <= i => p i)
+proof.
+  intros p hyp i iVal.
+  cut temp : (forall k, k > 0 => k <= i => p k).
+  apply (Induction.induction (lambda i, forall k, k > 0 => k <= i => p k) _ _ i _).
+  trivial.
+  simplify.
+  intros j hypRec hypJ.
+  trivial.
+  trivial.
+  trivial.
+save.
+
+op init2: int -> (int -> 'a) -> 'a array.
+
+axiom init2_length: forall (n:int, f:int -> 'a), n > 0 =>
+  length (init2 n f) = n.
+
+axiom init2_get: forall (n:int, i:int, f:int -> 'a),
+  0 <= i => i < n =>
+  (init2 n f).[i] = f i.
+
+  
+op range : int -> int -> 'a -> (int -> 'a -> 'a) -> 'a.
+
+axiom range_init :
+  forall (i j:int),
+    forall (x:'a),
+      forall (f:int -> 'a -> 'a),
+        j <= i => range i j x f = x.
+
+axiom range_ind :
+  forall (i j:int),
+    forall (x:'a),
+      forall (f:int -> 'a -> 'a),
+        i < j => (range i j x f = f j (range i (j-1) x f)).
+
+op appender(extract:int -> 'a array ->  'a, i:int, ar:'a array) : 'a array =
+  ar:::(extract (i-1) ar).
+
+op appendInit(ar:'a array, size:int, extract:int -> 'a array -> 'a) : 'a array =
+  let n = Array.length ar in
+  range n (n+size) ar (appender extract).
+
+lemma appendInit_length :
+  forall (ar:'a array) (n:int) (extract:int -> 'a array -> 'a),
+    n >= 0 =>
+    Array.length (appendInit ar n extract) = (Array.length ar) + n
+proof.
+  intros ar n extract hypN.
+  apply (
+    Induction.induction
+    (lambda (l:int), l <= n =>
+      (Array.length (appendInit ar l extract) = (Array.length ar) + l))
+    _ _ n _ _).
+  trivial.
+  intros j hypj hypRec hypJ2.
+  cut hyp : ((length ar) + j = length (appendInit ar (j-1) extract) + 1).
+  trivial.
+  rewrite hyp.
+  delta appendInit.
+  simplify.
+  cut temp : (
+    (range (length ar) ((+) (length ar) j) ar (appender extract)) =
+appender extract ((+) (length ar) j) (range (length ar) ((+) (length ar) ((-) j 1)) ar (appender extract))).
+  trivial.
+  trivial.
+  trivial.
+  trivial.
+save.
+
+
+lemma appendInit_ind :
+  forall (ar:'a array) (n:int) (extract:int -> 'a array -> 'a),
+    forall (k:int),
+      0 <= k /\ k < (Array.length ar) + n - 1 =>
+      n > 0 =>
+      (appendInit ar n extract).[k] = (appendInit ar (n-1) extract).[k]
+proof.
+  intros ar n extract k hypK hypN.
+  cut introVar : (
+     forall s,
+       s = (length ar)=>
+         (appendInit ar n extract).[k] = (appendInit ar ((-) n 1) extract).[k]
+  ).
+  intros s valS.
+  delta appendInit.
+  simplify.
+  rewrite <- valS.
+  cut lem : (
+    (range s (s+n) ar (appender extract)) =
+    (appender extract (s+n) (range s ((s+n)-1) ar (appender extract)))
+  ).
+  apply (range_ind<:'a array> s (s+n) ar (appender extract) _).
+  trivial.
+
+  rewrite lem.
+  cut temp : (forall ar, length ar = s+n-1 => (appender extract (s+n) ar).[k] = ar.[k]).
+  intros tar.
+  trivial.
+  rewrite (_:(s+n)-1=s+(n-1)).
+  trivial.
+  apply (temp (range s (s+(n-1)) ar (appender extract)) _).
+  cut test : (length (appendInit ar ((-) n 1) extract) = (length ar) + (n-1)).
+  apply (appendInit_length<:'a> ar (n-1) extract _).
+  trivial.
+  trivial.
+  trivial.
+save.
+
+lemma appendInit_get1 :
+  forall (ar:'a array) (n:int) (extract:int -> 'a array -> 'a),
+    forall (k:int),
+      0 <= k /\ k < Array.length ar =>
+      n >= 0 =>
+      (appendInit ar n extract).[k] = ar.[k]
+proof.
+  intros ar n extract k hypK hypN.
+  apply (
+    Induction.induction
+    (lambda (l:int), l <= n => (appendInit ar l extract).[k] = ar.[k])
+    _ _ n _ _);trivial.
+save.
+
+
+lemma appendInit_get2 :
+  forall (ar:'a array) (n:int) (extract:int -> 'a array -> 'a),
+    forall (k:int),
+      Array.length ar <= k /\ k < (Array.length ar) + n - 1 =>
+      n > 0 =>
+      (appendInit ar n extract).[k] = (extract k (appendInit ar (k-length ar) extract))
+proof.
+  intros ar n extract k hypK hypN.
+  rewrite (_: n = ((k-length ar)+1+(n-(k-length ar)-1)));[trivial|].
+  apply (Induction.induction
+    (lambda i, (appendInit ar ((k-length ar)+1+i) extract).[k] = (extract k (appendInit ar (k-length ar) extract)))
+    _ _ (n-(k-length ar)-1) _
+  );[|trivial|trivial].
+  simplify.
+  cut lem : ((appendInit ar (k-(length ar)+1) extract)
+    = appender extract (k+1) (appendInit ar (k-(length ar)) extract)
+  );trivial.
+save.
+
+lemma appendInit_getFinal :
+  forall (ar:'a array) (n:int) (extract:int -> 'a array -> 'a),
+    forall (k:int),
+      Array.length ar <= k /\ k < (Array.length ar) + n - 1 =>
+      n > 0 =>
+      extract k (appendInit ar n extract) = extract k (sub (appendInit ar n extract) 0 k) =>
+      (appendInit ar n extract).[k] = (extract k (appendInit ar n extract))
+proof.
+  intros ar n extract k hypK hypN hypExtract.
+  cut temp : ((appendInit ar n extract).[k] = (extract k (appendInit ar (k-length ar) extract))).
+  trivial.
+  rewrite temp.
+  cut temp2 : (sub (appendInit ar n extract) 0 k = appendInit ar (k-(length ar)) extract).
+  cut temp3 : (forall i, 0 <= i /\ i < k => (appendInit ar (k-(length ar)) extract).[i] = (appendInit ar n extract).[i]).
+  intros i hypI.
+  rewrite (_: n = ((+) ((-) n ((-) k (length ar))) ((-) k (length ar))) );[trivial|].
+  apply (Induction.induction
+    (lambda j,
+      j <= n - ((-) k (length ar)) =>
+      (appendInit ar ((-) k (length ar)) extract).[i] =
+        (appendInit ar (j+((-) k (length ar))) extract).[i]
+    ) _ _ (n - ((-) k (length ar))) _ _
+  );trivial.
+  apply (extentionality<:'a> (sub (appendInit ar n extract) 0 k) (appendInit ar ((-) k (length ar)) extract) _ ).
+  trivial.
+  trivial.
+save.
